QuickSort over NuPool: making sure the only thing missing is codeable for alive/done

share/pulse/examples/Quicksort.Task.NuPool.fst
@@ -32,23 +32,80 @@ open Quicksort.Base
 open Pulse.Lib.Par.Pledge
 
 let quicksort_post a lo hi s0 lb rb : vprop =
-  exists* s. (A.pts_to_range a lo hi s ** pure (pure_post_quicksort a lo hi lb rb s0 s))
+  op_exists_Star #(Seq.seq int) (FunctionalExtensionality.on (Seq.seq int) (fun s -> A.pts_to_range a lo hi s ** pure (pure_post_quicksort a lo hi lb rb s0 s)))
+  
+assume (* XXX, should be OK *)
+SmallPtsToRange : forall t (a : A.array t) lo hi s. is_small (A.pts_to_range a lo hi s)
+
+assume  (* XXX *)
+val codeable_pool_alive (p:T.pool) (f:perm) : codeable (poolcode Codeable.small_code) (T.pool_alive #f p)
+
+assume  (* XXX *)
+val codeable_pool_done (p:T.pool) : codeable (poolcode Codeable.small_code) (T.pool_done p)
 
 val cod1 (p:T.pool) (f:perm) (a:A.array int) (lo:nat) (hi:nat{lo <= hi}) (pivot:int) (s : erased (Seq.seq int)) (lb rb : erased int)
 : codeable (poolcode Codeable.small_code)
            (T.pool_alive #(half_perm f) p ** A.pts_to_range a lo hi s ** pure (pure_pre_quicksort a lo hi lb pivot s))
-let cod1 p f a lo hi pivot s lb rb =
-  magic()
-  // codeable_star _ _ _ _
-  // (codeable_star _ _ _ _ 
-  //   (magic ())
-  //   (codeable_small _ _))
-  // (codeable_small _ _)
 
-assume
+let cod1 p f a lo hi pivot s lb rb =
+  codeable_star _ _ _
+  (codeable_star _ _ _
+    (codeable_pool_alive p (half_perm f))
+    (codeable_base _ _ <| codeable_small _ _))
+  (codeable_base _ _ <| codeable_small _ (pure_is_small _))
+
+val codeable_qs_post (a:A.array int) (lo:nat) (hi:nat{lo <= hi}) (s0 : erased (Seq.seq int)) (lb rb : erased int)
+: codeable (poolcode Codeable.small_code)
+           (quicksort_post a lo hi s0 lb rb)
+
+let codeable_qs_post a lo hi s0 lb rb =
+  let open FStar.Tactics.V2 in
+  coerce_eq (_ by (trefl())) <|
+    codeable_exists2
+      Codeable.small_code
+      (Seq.seq int)
+      (fun s -> A.pts_to_range a lo hi s ** pure (pure_post_quicksort a lo hi lb rb s0 s))
+      (fun (x: Seq.seq int) -> codeable_star _ _ _
+                                  (codeable_base _ _ <| codeable_small _ _)
+                                  (codeable_base _ _ <| codeable_small _ <| pure_is_small _)
+                                  )
+
 val cod2 (p:T.pool) (f:perm) (a:A.array int) (lo:nat) (hi:nat{lo <= hi}) (s : erased (Seq.seq int)) (lb rb : erased int)
 : codeable (poolcode Codeable.small_code)
            (pledge [] (T.pool_done p) (T.pool_alive #(half_perm f) p ** quicksort_post a lo hi s lb rb))
+           
+let cod2 p f a lo hi s lb rb =
+  let open FStar.FunctionalExtensionality in
+  codeable_pledge _
+    _ (codeable_pool_done p)
+    _ (codeable_star _ _ _
+       (codeable_pool_alive p (half_perm f))
+       (codeable_qs_post a lo hi s lb rb))
+
+open FStar.Tactics.V2
+
+let op_exists_star_on_lem
+  (a : Type)
+  (f : a -> vprop)
+  : Lemma (op_exists_Star #a f == op_exists_Star #a (FunctionalExtensionality.on a f))
+          [SMTPat (op_exists_Star #a f)]
+  = admit() (* XXX *)
+
+let op_exists_star_on_lem2
+  (a : Type)
+  (f : a -> vprop)
+  : Lemma (op_exists_Star #a (FunctionalExtensionality.on a f) == op_exists_Star #a f)
+          [SMTPat (op_exists_Star #a f)]
+  = op_exists_star_on_lem a f
+
+let vprop_equiv_refl' (v0 v1 :vprop) (_ : squash (v0 == v1)) : vprop_equiv v0 v1 = vprop_equiv_refl v0
+
+let tac1 () : Tac unit =
+  apply (`vprop_equiv_refl');
+  apply_lemma (`op_exists_star_on_lem)
+let tac2 () : Tac unit =
+  apply (`vprop_equiv_refl');
+  apply_lemma (`op_exists_star_on_lem2)
 
 ```pulse
 fn rec t_quicksort
@@ -106,9 +163,30 @@ fn rec t_quicksort
         quicksort_post a lo hi s0 lb rb
     {
       (* Functional correctness *)
+
       unfold quicksort_post;
       unfold quicksort_post;
+
+      (* Removing the on_domain *)
+      rewrite_by
+        (op_exists_Star #(Seq.seq int) (FunctionalExtensionality.on (Seq.seq int) (fun s -> A.pts_to_range a lo r._1 s ** pure (pure_post_quicksort a lo r._1 lb pivot s1 s))))
+        (op_exists_Star #(Seq.seq int) (fun s -> A.pts_to_range a lo r._1 s ** pure (pure_post_quicksort a lo r._1 lb pivot s1 s)))
+        tac2
+        ();
+      rewrite_by
+        (op_exists_Star #(Seq.seq int) (FunctionalExtensionality.on (Seq.seq int) (fun s -> A.pts_to_range a r._2 hi s ** pure (pure_post_quicksort a r._2 hi pivot rb s3 s))))
+        (op_exists_Star #(Seq.seq int) (fun s -> A.pts_to_range a r._2 hi s ** pure (pure_post_quicksort a r._2 hi pivot rb s3 s)))
+        tac2
+        ();
+
       quicksort_proof a lo r._1 r._2 hi lb rb pivot #s0 s1 s2 s3;
+
+      rewrite_by
+        (op_exists_Star #(Seq.seq int) (fun s -> A.pts_to_range a lo hi s ** pure (pure_post_quicksort a lo hi lb rb s0 s)))
+        (op_exists_Star #(Seq.seq int) (FunctionalExtensionality.on (Seq.seq int) (fun s -> A.pts_to_range a lo hi s ** pure (pure_post_quicksort a lo hi lb rb s0 s))))
+        tac1
+        ();
+
       fold (quicksort_post a lo hi s0 lb rb);
 
       (* Permission accounting *)
@@ -118,9 +196,14 @@ fn rec t_quicksort
 
     ()
   } else {
+    rewrite_by
+      (op_exists_Star #(Seq.seq int) (fun s -> A.pts_to_range a lo hi s ** pure (pure_post_quicksort a lo hi lb rb s0 s)))
+      (op_exists_Star #(Seq.seq int) (FunctionalExtensionality.on (Seq.seq int) (fun s -> A.pts_to_range a lo hi s ** pure (pure_post_quicksort a lo hi lb rb s0 s))))
+      tac1
+      ();
     return_pledge [] (T.pool_done p) (
       T.pool_alive #f p **
-      (exists* s. A.pts_to_range a lo hi s ** pure (pure_post_quicksort a lo hi lb rb s0 s))
+      (op_exists_Star #(Seq.seq int) (FunctionalExtensionality.on (Seq.seq int) (fun s -> A.pts_to_range a lo hi s ** pure (pure_post_quicksort a lo hi lb rb s0 s))))
     );
   }
 }
